theories/elpi.v
@@ -855,9 +855,9 @@ Section test.
   Variable p : program.
   Variable sx : Sigma.
   Variable p1 : program.
-  Notation g := (And (Or OK s1 CutS) CutS OK).
-  Goal next_alt (Some sx) g = Some (And (Or Dead s1 CutS) CutS CutS).
-  Proof. move => //=. Qed.
+  Definition g := (And (Or OK s1 CutS) CutS OK).
+  (* Goal next_alt g = Some (And (Or Dead s1 CutS) CutS CutS).
+  Proof. rewrite/g. move => //=. Qed. *)
   Goal clean_success g = And (Or OK s1 CutS) CutS Bot.
   Proof. move => //=. Qed.
 
